theories/base_logic/lib/gen_heap.v
@@ -143,17 +143,17 @@ Section gen_heap.
   Qed.
 
   Lemma gen_heap_alloc_gen σ σ' :
-    σ ##ₘ σ' → gen_heap_ctx σ ==∗ gen_heap_ctx (σ ∪ σ') ∗ [∗ map] l ↦ v ∈ σ', l ↦ v.
+    σ ##ₘ σ' → gen_heap_ctx σ ==∗ gen_heap_ctx (σ' ∪ σ) ∗ [∗ map] l ↦ v ∈ σ', l ↦ v.
   Proof.
     revert σ; induction σ' as [| l v σ' Hl IHσ'] using map_ind;
       iIntros (σ Hσdisj) "Hσ".
-    - by rewrite right_id big_opM_empty; iFrame.
+    - by rewrite left_id big_opM_empty; iFrame.
     - iMod (IHσ' with "Hσ") as "[Hσ m]"; first by eapply map_disjoint_insert_r.
       rewrite big_opM_insert //; iFrame.
       assert (σ !! l = None).
       { eapply map_disjoint_Some_r; first by eauto.
         rewrite lookup_insert //. }
-      rewrite -insert_union_r //.
+      rewrite -insert_union_l //.
       iMod (gen_heap_alloc with "Hσ") as "[$ $]"; last done.
       apply lookup_union_None; split; auto.
   Qed.
